\loesung{

First, recall that the formula for the coefficient of determination $R^2$ is:
\begin{align*}
	R^2 = 1-\frac{SSE_{LM}}{SSE_{c}}
\end{align*}
where $SSE_{LM} = \sum_{i=1}^n (y^{(i)} - \hat{f}_{LM}(x^{(i)}))^2$ is the sum of squares due to regression and $SSE_{c} = \sum_{i=1}^n (y^{(i)} - \bar{y})^2$ is the total sum of squares. The formula for the Pearson correlation coefficient $\rho$ is:
\begin{align*}
	\rho(x, y) = \frac{cov(x, y)}{\sigma_{x}\sigma_{y}} 
	= \frac{\sum_{i=1}^{n}{(x^{(i)}-\bar{x}) \cdot (y^{(i)}-\bar{y})}}{\sqrt{\sum_{i=1}^{n}(x^{(i)}-\bar{x})^2} \sqrt{\sum_{i=1}^{n}{(y^{(i)}-\bar{y})^2 }}}.
\end{align*}
We have:
\begin{align*}
	R^2 &= 1-\frac{SSE_{LM}}{SSE_{c}} \\
	&= 1 - \frac{\sum_{i=1}^n (y^{(i)} - \hat{f}_{LM}(x^{(i)}))^2}{\sum_{i=1}^n (y^{(i)} - \bar{y})^2} \\
	&= 1 - \frac{\sum_{i=1}^n (y^{(i)} - \hat{y}^{(i)})^2}{\sum_{i=1}^n (y^{(i)} - \bar{y})^2} 
\end{align*}
Similarly, we can write:
\begin{align*}
	\rho^2 &= \left(\frac{\mathrm{cov}(X,Y)}{\sigma_X\sigma_Y}\right)^2 \\
	&= \left(\frac{\sum_{i=1}^n (x^{(i)} - \bar{x})(y^{(i)} - \bar{y})}{\sqrt{\sum_{i=1}^n (x^{(i)} - \bar{x})^2}\sqrt{\sum_{i=1}^n (y^{(i)} - \bar{y})^2}}\right)^2 \\
	&= \frac{\left(\sum_{i=1}^n (x^{(i)} - \bar{x})(y^{(i)} - \bar{y})\right)^2}{\left(\sum_{i=1}^n (x^{(i)} - \bar{x})^2\right)\left(\sum_{i=1}^n (y^{(i)} - \bar{y})^2\right)}\\
	&= \frac{\left(\sum_{i=1}^n (x^{(i)} - \bar{x})(y^{(i)} - \bar{y})\right)^2}{\left(\sum_{i=1}^n (x^{(i)} - \bar{x})^2\right)\left(\sum_{i=1}^n (y^{(i)} - \bar{y})^2\right)} \frac{\sum_{i=1}^n (x^{(i)} - \bar{x})^2}{\sum_{i=1}^n (x^{(i)} - \bar{x})^2}\\
	&= \left(\frac{\sum_{i=1}^n (x^{(i)} - \bar{x})(y^{(i)} - \bar{y})}{\sum_{i=1}^n (x^{(i)} - \bar{x})^2}\right)^2 \frac{\sum_{i=1}^n (x^{(i)} - \bar{x})^2}{\sum_{i=1}^n (y^{(i)} - \bar{y})^2} \\
	&= \hat{\beta}_1^2 \, \frac{\sum_{i=1}^n (x^{(i)} - \bar{x})^2}{\sum_{i=1}^n (y^{(i)} - \bar{y})^2}
\end{align*}

Now, note that

\begin{align*}
	\sum_{i=1}^n (y^{(i)}-\bar{y})^2 &= \sum_{i=1}^n (y^{(i)}-\hat{y}^{(i)})^2 + \sum_{i=1}^n (\hat{y}^{(i)} - \bar{y})^2.
\end{align*}
Proof: 
\begin{align*}
	\sum_{i=1}^n (y^{(i)}-\bar{y})^2 
	&= \sum_{i=1}^n (y^{(i)} - \hat{y}^{(i)} + \hat{y}^{(i)} - \bar{y})^2 \\
	&= \sum_{i=1}^n (y^{(i)} - \hat{y}^{(i)})^2 + (\hat{y}^{(i)} - \bar{y})^2 + 2(y^{(i)}-\hat{y}^{(i)})(\hat{y}^{(i)} - \bar{y}) \\
	&= \sum_{i=1}^n (y^{(i)} - \hat{y}^{(i)})^2 + \sum_{i=1}^n(\hat{y}^{(i)} - \bar{y})^2 + 2\sum_{i=1}^n(y^{(i)}-\hat{y}^{(i)})(\hat{y}^{(i)} - \bar{y})
\end{align*}
It remains to show that 
\begin{align*}
	2\sum_{i=1}^n(y^{(i)}-\hat{y}^{(i)})(\hat{y}^{(i)} - \bar{y}) &= 0 \\
	\sum_{i=1}^n (y^{(i)}-\hat{y}^{(i)})\hat{y}^{(i)} - \sum_{i=1}^n (y^{(i)}-\hat{y}^{(i)})\bar{y}&= 0 \\
	\bar{y}\, \sum_{i=1}^n y^{(i)}-\hat{y}^{(i)} &= 0 \\
	\sum_{i=1}^n y^{(i)}-\hat{y}^{(i)} &= 0
\end{align*}

where we have used the fact that $\sum_{i=1}^n (y^{(i)}-\hat{y}^{(i)})\hat{y}^{(i)} = 0$ as the residuals $(y^{(i)}-\hat{y}^{(i)})$ and $\hat{y}^{(i)}$ are not correlated.

Substituting these results into the expression for $R^2$, we obtain:

\begin{align*}
	R^2 &= 1 - \frac{\sum_{i=1}^n (y^{(i)} - \hat{y}^{(i)})^2}{\sum_{i=1}^n (y^{(i)} - \bar{y})^2} \\
	&= \frac{\sum_{i=1}^n (y^{(i)} - \bar{y})^2 - \sum_{i=1}^n (y^{(i)} - \hat{y}^{(i)})^2}{\sum_{i=1}^n (y^{(i)} - \bar{y})^2}\\
	&= \frac{\sum_{i=1}^n (y^{(i)}-\hat{y}^{(i)})^2 + \sum_{i=1}^n (\hat{y}^{(i)} - \bar{y})^2 - \sum_{i=1}^n (y^{(i)} - \hat{y}^{(i)})^2}{\sum_{i=1}^n (y^{(i)} - \bar{y})^2}\\
	&= \frac{\sum_{i=1}^n (\hat{y}^{(i)} - \bar{y})^2}{\sum_{i=1}^n (y^{(i)} - \bar{y})^2}\\
	&= \frac{\sum_{i=1}^n(\hat{\beta}_0 + \hat{\beta}_1 x^{(i)}- (\hat{\beta}_0 + \hat{\beta}_1 \bar{x}))^2}{\sum_{i=1}^n (y^{(i)} - \bar{y})^2} \\
	&= \frac{\hat{\beta}_1^2 \sum_{i=1}^n (x^{(i)} - \bar{x})^2}{\sum_{i=1}^n (y^{(i)} - \bar{y})^2} \\
	&= \rho^2
\end{align*}

Hence, we have shown that $R^2 = \rho^2$, which completes the proof. Note that this result is valid only for simple linear regression, where there is only one independent variable. For multiple regression, the coefficient of determination is defined differently and does not necessarily equal the square of the Pearson correlation coefficient.

}
